src/Examples/Tutorial/Tutorial.v
@@ -21,3 +21,75 @@ Export Fiat.QueryStructure.Automation.AutoDB
         Fiat.QueryStructure.Automation.SearchTerms.FindPrefixSearchTerms.
 
 Ltac pick := erewrite refine_pick_val by eauto.
+
+Hint Resolve refine_pick_val.
+Hint Rewrite <- app_nil_end.
+
+Definition testnil A B (ls : list A) (cnil ccons : B) : B :=
+  match ls with
+  | nil => cnil
+  | _ :: _ => ccons
+  end.
+
+Lemma refine_testnil : forall A (ls : list A) B (c1 cnil ccons : Comp B),
+  (ls = nil -> refine c1 cnil)
+  -> (ls <> nil -> refine c1 ccons)
+  -> refine c1 (testnil ls cnil ccons).
+Proof.
+  destruct ls; intuition congruence.
+Qed.
+
+Add Parametric Morphism A B
+: (@testnil A (Comp B))
+    with signature
+    @eq (list A)
+      ==> @refine B
+      ==> @refine B
+      ==> @refine B
+      as refine_testnil_morphism.
+Proof.
+  destruct y; auto.
+Qed.
+
+Lemma refine_testnil_ret : forall A B (ls : list A) (cnil ccons : B),
+  refine (testnil ls (ret cnil) (ret ccons)) (ret (testnil ls cnil ccons)).
+Proof.
+  destruct ls; reflexivity.
+Qed.
+
+Ltac refine_testnil ls' := etransitivity; [ apply refine_testnil with (ls := ls'); intro | ].
+
+Definition let_ A B (v : A) (f : A -> B) := let x := v in f v.
+
+Add Parametric Morphism A B
+: (@let_ A (Comp B))
+    with signature
+    @eq A
+      ==> pointwise_relation _ (@refine B)
+      ==> @refine B
+      as refine_let_morphism.
+Proof.
+  unfold pointwise_relation, let_; auto.
+Qed.
+
+Lemma refine_let : forall A B (v : A) c1 (c2 : A -> Comp B),
+  (forall x, x = v -> refine c1 (c2 x))
+  -> refine c1 (let_ v c2).
+Proof.
+  unfold let_; auto.
+Qed.
+
+Ltac refine_let := apply refine_let.
+
+Lemma refine_let_ret : forall A B (v : A) (f : A -> B),
+  let_ v (fun x => ret (f x)) =  ret (let_ v f).
+Proof.
+  reflexivity.
+Qed.
+
+Ltac monad_simpl := autosetoid_rewrite with refine_monad; simpl.
+
+Hint Rewrite refine_let_ret refine_testnil_ret : cleanup.
+
+Ltac cleanup := autorewrite with cleanup.
+Ltac finalize := finish_SharpeningADT_WithoutDelegation.
